We use Defined instead of Qed

proofs.v
@@ -14,13 +14,6 @@ Inductive Correctness : Type :=
 | trusted : Correctness
 | idk : Correctness.
 
-Inductive ComparableNode : Type :=
-  mkComparableNode
-    {
-      ComparableNodeContent : string
-    ; ComparableNodeChildren : list ComparableNode
-    }.
-
 Inductive Node : Type :=
   mkNode
     {
@@ -28,17 +21,6 @@ Inductive Node : Type :=
     ;correctness : Correctness
     ; children : list Node
     }.
-
-Fixpoint get_comparable_node_from_node (n: Node) : ComparableNode :=
-  mkComparableNode (content n) (map (fun child => get_comparable_node_from_node child) (children n)).
-
-Lemma comparable_node_content_eq_to_node_content : forall n:Node, content n = ComparableNodeContent (get_comparable_node_from_node n).
-Proof.
-  intros n.
-  induction n.
-  simpl.
-  reflexivity.
-Qed.
 
 Fixpoint or_list (l : list Prop) : Prop :=
   match l with
@@ -55,7 +37,7 @@ Proof.
   intuition.
   rewrite <- H0.
   exact H1.
-Qed.
+Defined.
 
 Lemma node_is_in_itself : forall n : Node, is_node_in_tree (content n) n.
 Proof.
@@ -64,7 +46,7 @@ Proof.
   simpl.
   left.
   + reflexivity.
-Qed.
+Defined.
 
 Lemma head_of_non_empty_children_is_in_parent : forall parent child : Node, (children parent) <> nil /\ hd (mkNode "I don't exist"%string idk nil) (children parent) = child -> is_node_in_tree (content child) parent.
 Proof.
@@ -82,7 +64,7 @@ Proof.
     left.
     rewrite H.
     apply node_is_in_itself.
-Qed.
+Defined.
 
 Lemma child_node_is_in_parent : forall parent child : Node, In child (children parent) -> is_node_in_tree (content child) parent.
 Proof.
@@ -113,12 +95,11 @@ Proof.
     simpl.
     right.
     exact H1.
-Qed.
+Defined.
 
 Definition node1 := mkNode "node1"%string idk nil.
 Definition node2 := mkNode "node2"%string idk nil.
 Definition node3 := mkNode "node3"%string trusted (node1::node2::nil).
-Eval compute in get_comparable_node_from_node node1 = get_comparable_node_from_node node1.
 Eval compute in correctness node3.
 
 Lemma list_sum_ge_0 : forall l : list nat, 0 <= list_sum l.
@@ -136,7 +117,7 @@ Proof.
   induction a.
   intuition.
   intuition.
-Qed.
+Defined.
 
 Fixpoint and_list (l : list Prop) : Prop :=
   match l with
@@ -155,7 +136,7 @@ Proof.
       inversion H0.
       exact H.
     - inversion H0. intuition.
-Qed.
+Defined.
 
 Fixpoint weight (node : Node) : nat :=
   match children node with
@@ -172,7 +153,7 @@ Proof.
   exact H.
   rewrite H0.
   reflexivity.
-Qed.
+Defined.
 
 Lemma weight_gt_0: forall n:Node, 0 < weight n.
 Proof.
@@ -183,7 +164,7 @@ Proof.
     intuition.
   + simpl.
     intuition.
-Qed.
+Defined.
 
 Lemma node_weight_gt_sum_children_weight: forall n:Node, weight n > list_sum (map (fun child => weight child) (children n)).
 Proof.
@@ -197,7 +178,7 @@ Proof.
     exact l.
   + simpl.
     intuition.
-Qed.
+Defined.
 
 Lemma nat_in_list_le_list_sum: forall (l:list nat) (element: nat), In element l -> element <= list_sum l.
 Proof.
@@ -212,7 +193,7 @@ Proof.
     - transitivity (list_sum l);auto.
       rewrite Nat.add_comm.
       apply Nat.le_add_r.
-Qed.
+Defined.
 
 Lemma child_weight_le_sum_children_weight: forall (l:list Node) (child: Node), In child l -> list_sum (map (fun child => weight child) l) >= weight child.
 Proof.
@@ -227,7 +208,7 @@ Proof.
       intuition.
     + subst.
       intuition.
-Qed.
+Defined.
 
 Lemma parent_weight_gt_child_weight: forall parent child:Node, In child (children parent) -> weight child < weight parent.
 Proof.
@@ -255,7 +236,7 @@ Proof.
     rewrite Nat.add_comm.
     intuition.
     intuition.
-Qed.
+Defined.
 
 Fixpoint are_all_idk (node : Node) : Prop :=
   and (node.(correctness) = idk) (and_list (map (fun child => are_all_idk child) (children node))).
@@ -274,7 +255,7 @@ Proof.
   - inversion H.
     apply H3.
   - apply H1.
-Qed.
+Defined.
 
 Eval compute in are_all_idk node1.
 Definition node4 := mkNode "node4"%string idk (node1::node2::nil).
@@ -290,7 +271,7 @@ Proof.
   split.
   + exact H0.
   + exact H1.
-Qed.
+Defined.
   (* Extraction pred. *)
 (* Extraction is_debugging_tree. *)
 
@@ -341,22 +322,12 @@ Definition my_node_list : list Node := node1::node2::node3::node4::node5::nil.
 Eval compute in list_max (nil).
 (* Goal 0 * 0 = 2 -> False. *)
 (* Proof. easy. *)
-(* Qed. *)
+(* Defined. *)
 
 Definition evaluate_node (n : Node) : Correctness :=
   no.
-(* Lemma largest_of_list_is_correct: forall l: list nat, l <> nil -> get_largest_nat_in_list l <> nil. *)
-(* Proof. intros l H. induction l. intuition. induction a. intuition. exact: (False_ind (0::l = [])). *)
-(* Qed. *)
-(* Definition get_heaviest_node (l : list Node, n : nat) : (bool * Node) := *)
-(*   match l with *)
-(*     nil => (false, mkNode idk nil) *)
-(*     | *)
-(* Definition heaviest_first_strategy (n : {n : Node | eq_true (andb (is_debugging_tree n) (Nat.ltb 0 (length (children n))))}) : Node := *)
-(*   (hd (mkNode idk nil) (children (proj1_sig n))). *)
-(* Eval compute in top_down_strategy node5. *)
-(* Scheme Equality for Node. *)
-(* Eval compute in Node_beq (mkNode no nil) (mkNode no nil). *)
+
+
 Definition get_debugging_tree_from_tree (n : Node) : Node :=
   mkNode (content n) no (children n).
 Require Import Program.Wf.
@@ -366,7 +337,7 @@ Proof.
   induction n.
   simpl.
   reflexivity.
-Qed.
+Defined.
 
 Lemma children_of_debugging_tree_remain_unchanged: forall n:Node, children n = children (get_debugging_tree_from_tree n).
 Proof.
@@ -374,7 +345,7 @@ Proof.
   induction n.
   simpl.
   reflexivity.
-Qed.
+Defined.
 
 Lemma debugging_tree_root_node_is_incorrect: forall n:Node, correctness (get_debugging_tree_from_tree n) = no.
 Proof.
@@ -382,7 +353,7 @@ Proof.
   induction n.
   simpl.
   reflexivity.
-Qed.
+Defined.
 
 Lemma debugging_tree_of_tree_with_all_children_idk_is_debugging_tree: forall n:Node, and_list (map (fun child => are_all_idk child) (children n)) -> is_debugging_tree (get_debugging_tree_from_tree n).
 Proof.
@@ -397,7 +368,7 @@ Proof.
        + unfold is_debugging_tree. split.
          - exact H1.
          - exact H2.
-Qed.
+Defined.
 Require Import Lia.
 
 Lemma debugging_tree_of_idk_tree_is_debugging_tree: forall n:Node, are_all_idk n -> is_debugging_tree (get_debugging_tree_from_tree n).
@@ -413,16 +384,7 @@ Proof.
     apply children_of_debugging_tree_remain_unchanged.
     rewrite <- H1.
     exact H0.
-Qed.
-SearchPattern (_ = _ -> _ = _).
-
-Lemma comparable_node_of_debugging_tree_of_tree_is_comparable_node: forall n:Node, get_comparable_node_from_node (get_debugging_tree_from_tree n) = get_comparable_node_from_node n.
-Proof.
-  intros n.
-  induction n.
-  simpl.
-  reflexivity.
-Qed.
+Defined.
 
 Lemma debugging_tree_of_tree_is_in_tree: forall n:Node, is_node_in_tree (content (get_debugging_tree_from_tree n)) n.
 Proof.
@@ -431,7 +393,7 @@ Proof.
   simpl.
   left.
   reflexivity.
-Qed.
+Defined.
 
 
 Lemma content_debugging_tree_eq_content_tree: forall n:Node, content (get_debugging_tree_from_tree n) = content n.
@@ -440,7 +402,7 @@ Proof.
   induction n.
   simpl.
   reflexivity.
-Qed.
+Defined.
 
 Lemma children_head_of_debugging_tree_are_all_idk: forall (n head:Node) (tail: list Node), children n = head::tail /\ is_debugging_tree n -> are_all_idk head.
 Proof.
@@ -459,7 +421,7 @@ Proof.
       left.
       inversion H0.
       reflexivity.
-Qed.
+Defined.
 
 
 Lemma debugging_tree_of_children_head_of_debugging_tree_is_debugging_tree: forall (n head:Node) (tail: list Node), children n = head::tail /\ is_debugging_tree n -> is_debugging_tree (get_debugging_tree_from_tree head).
@@ -468,21 +430,13 @@ Proof.
   inversion H.
   inversion H1.
   assert (are_all_idk head).
-  + apply children_head_of_debugging_tree_are_all_idk with n.
+  + apply children_head_of_debugging_tree_are_all_idk with (n := n) (tail := tail).
     split.
-    - exact H3.
-    - induction n.
-      induction children0.
-      intuition.
-      simpl.
-      inversion H4.
-      simpl.
-      left.
-      inversion H0.
-      reflexivity.
+    - exact H0.
+    - exact H1.
   + apply debugging_tree_of_idk_tree_is_debugging_tree.
     exact H4.
-Qed.
+Defined.
 
 Obligation Tactic := intros.
 
@@ -504,34 +458,22 @@ Next Obligation.
     - rewrite <- H0.
       apply parent_weight_gt_child_weight.
       exact H.
-Qed.
+Defined.
 
 Next Obligation.
   intuition.
-Qed.
+Defined.
 
-(* Lemma gda_correct : forall n:Node, is_debugging_tree n -> is_debugging_tree (generic_debugging_algorithm_non_dependently_typed n) /\ children (generic_debugging_algorithm_non_dependently_typed n) = nil /\ is_node_in_tree (content (generic_debugging_algorithm_non_dependently_typed n)) n. *)
-(* Proof. *)
-(*   intros. *)
-(*   intuition. *)
-(*   + induction n. *)
-(*     induction children0. *)
-(*     - simpl. *)
-(*     intuition. *)
-(*     Tactics.program_simpl. *)
-(*     unfold generic_debugging_algorithm_non_dependently_typed. *)
-(*     simpl. *)
-(*     intuition. *)
 Obligation Tactic := intros.
 Obligation Tactic := Tactics.program_simpl.
 
-
-Program Fixpoint generic_debugging_algorithm_dependently_typed (n : {n: Node | is_debugging_tree n}) {measure (weight n)}: {m: Node | is_debugging_tree m /\ children m = nil} :=
+Program Fixpoint generic_debugging_algorithm_dependently_typed (n : {n: Node | is_debugging_tree n}) {measure (weight n)}: {m: Node | is_debugging_tree m} :=
   match children n with
     nil => n
   | head::tail => generic_debugging_algorithm_dependently_typed (get_debugging_tree_from_tree head)
   end.
-Print generic_debugging_algorithm_dependently_typed_obligation_1.
+
+Print generic_debugging_algorithm_dependently_typed_obligation_3.
 Next Obligation.
   inversion H.
   assert (are_all_idk head).
@@ -548,9 +490,12 @@ Next Obligation.
     exact H2.
     + apply debugging_tree_of_idk_tree_is_debugging_tree.
       exact H2.
-Qed.
+Defined.
+
 Obligation Tactic := intros.
+(* Proof about the weight *)
 Next Obligation.
+  simpl.
   assert (In head (children (proj1_sig n))).
   + induction (children (proj1_sig n)).
     - inversion Heq_anonymous.
@@ -564,27 +509,23 @@ Next Obligation.
       assert (match head.(children) with | [] => 1 | n0 :: l => S (weight n0 + list_sum (map (fun child : Node => weight child) l)) end = weight (get_debugging_tree_from_tree head)). intuition. rewrite H1. rewrite <- H0.
       apply parent_weight_gt_child_weight.
       exact H.
-Qed.
+Defined.
 
+Print generic_debugging_algorithm_dependently_typed_obligation_1.
+Print generic_debugging_algorithm_dependently_typed_obligation_2.
+Print generic_debugging_algorithm_dependently_typed_obligation_3.
 Obligation Tactic := intros.
 
-Program Fixpoint generic_debugging_algorithm_dp (n : {n: Node | is_debugging_tree n}) {measure (weight n)}: {m: Node | is_node_in_tree (content m) n /\ is_debugging_tree m /\ children m = nil} :=
+Program Fixpoint generic_debugging_algorithm_dependently_typed1 (n : {n: Node | is_debugging_tree n}) {measure (weight n)}: {m: Node | is_debugging_tree m /\ children m = nil} :=
   match children n with
     nil => n
-  | head::tail => generic_debugging_algorithm_dp (get_debugging_tree_from_tree head)
+  | head::tail => generic_debugging_algorithm_dependently_typed1 (get_debugging_tree_from_tree head)
   end.
-Obligations of generic_debugging_algorithm_dp.
+
+Obligation Tactic := Tactics.program_simpl.
 Solve All Obligations.
-Next Obligation.
-  simpl.
-  Tactics.program_simpl.
-  split.
-  + apply node_is_in_itself.
-  + split.
-    - exact H.
-    - reflexivity.
-Qed.
-Obligations of generic_debugging_algorithm_dp.
+Obligation Tactic := intros.
+Solve All Obligations.
 Next Obligation.
   Tactics.program_simpl.
   inversion H.
@@ -602,9 +543,161 @@ Next Obligation.
     exact H2.
     + apply debugging_tree_of_idk_tree_is_debugging_tree.
       exact H2.
-Qed.
+Defined.
+Solve All Obligations.
 Obligation Tactic := intros.
-Obligations of generic_debugging_algorithm_dp.
+Solve All Obligations.
+Next Obligation.
+  simpl.
+  assert (In head (children (proj1_sig n))).
+  + induction (children (proj1_sig n)).
+    - inversion Heq_anonymous.
+    - simpl.
+      left.
+      injection Heq_anonymous.
+      intuition.
+  + assert (weight head = weight (get_debugging_tree_from_tree head)).
+    - apply debugging_tree_of_tree_has_same_weight.
+    - simpl.
+      assert (match head.(children) with | [] => 1 | n0 :: l => S (weight n0 + list_sum (map (fun child : Node => weight child) l)) end = weight (get_debugging_tree_from_tree head)). intuition. rewrite H1. rewrite <- H0.
+      apply parent_weight_gt_child_weight.
+      exact H.
+Defined.
+
+Print generic_debugging_algorithm_dependently_typed1_obligation_1.
+Print generic_debugging_algorithm_dependently_typed1_obligation_2.
+Print generic_debugging_algorithm_dependently_typed1_obligation_3.
+Print generic_debugging_algorithm_dependently_typed1_obligation_4.
+(* Lemma generic_debugging_algorithm_dependently_typed1_returns_node_in_original_tree: forall n:Node, is_debugging_tree n -> is_node_in_tree (content (generic_debugging_algorithm_dependently_typed1 (proj1_sig n))) n. *)
+
+(* Next Obligation. *)
+(*   simpl. *)
+(*   assert (In head (children (proj1_sig n))). *)
+(*   + induction (children (proj1_sig n)). *)
+(*     - inversion Heq_anonymous. *)
+(*     - simpl. *)
+(*       left. *)
+(*       injection Heq_anonymous. *)
+(*       intuition. *)
+(*   + assert (weight head = weight (get_debugging_tree_from_tree head)). *)
+(*     - apply debugging_tree_of_tree_has_same_weight. *)
+(*     - simpl. *)
+(*       assert (match head.(children) with | [] => 1 | n0 :: l => S (weight n0 + list_sum (map (fun child : Node => weight child) l)) end = weight (get_debugging_tree_from_tree head)). *)
+(*       intuition. *)
+(*       rewrite H1. *)
+(*       rewrite <- H0. *)
+(*       apply parent_weight_gt_child_weight. *)
+(*       exact H. *)
+(* Defined. *)
+(* Solve All Obligations. *)
+(* Obligation Tactic := Tactics.program_simpl. *)
+(* Solve All Obligations. *)
+(* Obligation Tactic := intros. *)
+(* Solve All Obligations. *)
+(* Obligations of generic_debugging_algorithm_dependently_typed2. *)
+(* Solve All Obligations. *)
+(* Next Obligation. *)
+(*   simpl. *)
+(*   Tactics.program_simpl. *)
+(*   assert (are_all_idk head). *)
+(*     - apply children_head_of_debugging_tree_are_all_idk with (n:=n) (tail:=tail). *)
+(*       split. *)
+(*       + rewrite Heq_anonymous. *)
+(*         reflexivity. *)
+(*       + exact H. *)
+(*     - assert (content (get_debugging_tree_from_tree head) = content head). *)
+(*       + apply content_debugging_tree_eq_content_tree. *)
+(*         + split. *)
+(*           apply nodes_with_same_content with head. *)
+(*           split. *)
+(*           fold generic_debugging_algorithm_dependently_typed2_obligation_3. *)
+(*           fold generic_debugging_algorithm_dependently_typed2_obligation_1. *)
+(*           fold generic_debugging_algorithm_dependently_typed2_obligation_2. *)
+(*           fold generic_debugging_algorithm_dependently_typed2_obligation_5. *)
+(*           simpl. *)
+(*           Tactics.program_simpl. *)
+(*           simpl. *)
+(*           Tactics.program_simpl. *)
+(*           rewrite <- H1. *)
+(*       apply child_node_is_in_parent. *)
+(*       intuition. *)
+(*       split. *)
+
+(*       intuition. *)
+(*       exact Heq_anonymous. *)
+(*   assert (In head (children (proj1_sig n))). *)
+(*   - induction (children (proj1_sig n)). *)
+(*     + inversion Heq_anonymous. *)
+(*     + simpl. *)
+(*       left. *)
+(*       injection Heq_anonymous. *)
+(*       intuition. *)
+(*   - assert (content (get_debugging_tree_from_tree head) = content head). *)
+(*     apply content_debugging_tree_eq_content_tree. *)
+(*     assert (is_node_in_tree (content head) (proj1_sig n)). *)
+(*     apply child_node_is_in_parent. *)
+(*     exact H. *)
+(*     inversion H0. *)
+(*     assert (content head = content (get_debugging_tree_from_tree head)). *)
+(*     apply H0. *)
+(*     simpl. *)
+(*     assert (are_all_idk head). *)
+(*     + induction (children (proj1_sig n)). *)
+(*       inversion Heq_anonymous. *)
+(*       simpl. *)
+(*       injection Heq_anonymous. *)
+(*       intuition. *)
+(*       apply and_list_true_implies_element_in_list_true with (children (proj1_sig n)). *)
+(*       split. *)
+(* Defined. *)
+
+
+
+Program Fixpoint generic_debugging_algorithm_dependently_typed2 (n : {n: Node | is_debugging_tree n}) {measure (weight n)}: {m: Node | is_node_in_tree (content m) n /\ is_debugging_tree m /\ children m = nil} :=
+  match children n with
+    nil => n
+  | head::tail => generic_debugging_algorithm_dependently_typed2 (get_debugging_tree_from_tree head)
+  end.
+Obligations of generic_debugging_algorithm_dependently_typed2.
+Obligation Tactic := Tactics.program_simpl.
+Solve All Obligations.
+Obligation Tactic := intros.
+Solve All Obligations.
+Next Obligation.
+  simpl.
+  Tactics.program_simpl.
+  split.
+  + apply node_is_in_itself.
+  + split.
+    - exact H.
+    - reflexivity.
+Defined.
+Obligations of generic_debugging_algorithm_dependently_typed2.
+Solve All Obligations.
+Obligation Tactic := Tactics.program_simpl.
+Solve All Obligations.
+Next Obligation.
+  Tactics.program_simpl.
+  inversion H.
+  assert (are_all_idk head).
+  + assert (In head (children n)).
+  - induction (children n).
+    inversion Heq_anonymous.
+    simpl.
+    left.
+    injection Heq_anonymous.
+    intuition.
+  - apply and_list_true_implies_element_in_list_true with (children n).
+    split.
+    exact H1.
+    exact H2.
+    + apply debugging_tree_of_idk_tree_is_debugging_tree.
+      exact H2.
+Defined.
+Solve All Obligations.
+Obligation Tactic := intros.
+Solve All Obligations.
+Obligations of generic_debugging_algorithm_dependently_typed2.
 Next Obligation.
   assert (In head (children (proj1_sig n))).
   + induction (children (proj1_sig n)).
@@ -622,12 +715,43 @@ Next Obligation.
       rewrite <- H0.
       apply parent_weight_gt_child_weight.
       exact H.
-Qed.
-Obligation Tactic := simpl.
-Obligations of generic_debugging_algorithm_dp.
+Defined.
+Solve All Obligations.
+Obligation Tactic := Tactics.program_simpl.
+Solve All Obligations.
+Obligation Tactic := intros.
+Solve All Obligations.
+Obligations of generic_debugging_algorithm_dependently_typed2.
+Solve All Obligations.
 Next Obligation.
   simpl.
-  split.
+  Tactics.program_simpl.
+  assert (are_all_idk head).
+    - apply children_head_of_debugging_tree_are_all_idk with (n:=n) (tail:=tail).
+      split.
+      + rewrite Heq_anonymous.
+        reflexivity.
+      + exact H.
+    - assert (content (get_debugging_tree_from_tree head) = content head).
+      + apply content_debugging_tree_eq_content_tree.
+        + split.
+          apply nodes_with_same_content with head.
+          split.
+          fold generic_debugging_algorithm_dependently_typed2_obligation_1.
+          fold generic_debugging_algorithm_dependently_typed2_obligation_2.
+          fold generic_debugging_algorithm_dependently_typed2_obligation_3.
+          fold generic_debugging_algorithm_dependently_typed2_obligation_5.
+          simpl.
+          Tactics.program_simpl.
+          simpl.
+          Tactics.program_simpl.
+          rewrite <- H1.
+      apply child_node_is_in_parent.
+      intuition.
+      split.
+
+      intuition.
+      exact Heq_anonymous.
   assert (In head (children (proj1_sig n))).
   - induction (children (proj1_sig n)).
     + inversion Heq_anonymous.
@@ -652,4 +776,4 @@ Next Obligation.
       intuition.
       apply and_list_true_implies_element_in_list_true with (children (proj1_sig n)).
       split.
-Qed.
+Defined.
